src/Solver/TD_Interface.thy
@@ -1,5 +1,6 @@
 theory TD_Interface
-  imports TD_CFG_Core "TD.TD_plain" Constraint_System_Sound
+  imports TD_CFG_Core TD_CFG_IP_Core "TD.TD_plain" Constraint_System_Sound
+          Constraint_System_IP_Sound IMP2_Proc_to_CFG
 begin
 
 (* Plain TD backend (join only, no widening). *)
@@ -128,6 +129,202 @@ proof -
   interpret plain: td_cfg_plain_solver "to_cfg c" tf join_abs bot_abs s0 .
   show ?thesis
     unfolding td_analyse_def plain.td_env_at_def plain.td_sigma_at_def plain.cfg_T_def by simp
+qed
+
+(* -- Interprocedural TD backend (M1 slice 4) ----------------------- *)
+
+locale td_cfg_ip_solver = td_cfg_ip_core + TD_plain cfg_T_ip
+begin
+
+definition td_sigma_at :: "pp \<Rightarrow> (pp, 'a abs_state) map"
+where
+  "td_sigma_at v0 = TD_plain_Interp_solve cfg_T_ip v0"
+
+definition td_env_at :: "pp \<Rightarrow> pp \<Rightarrow> 'a abs_state"
+where
+  "td_env_at v0 w = lookup_bot (td_sigma_at v0) w"
+
+lemma td_sigma_at_solve:
+  "TD_plain_Interp_solve cfg_T_ip v0 = td_sigma_at v0"
+  unfolding td_sigma_at_def by simp
+
+lemma td_plain_part_solution_at:
+  assumes dom: "TD_plain.solve_dom cfg_T_ip v0"
+  shows "part_solution cfg_T_ip v0 (td_sigma_at v0) (reach cfg_T_ip (td_sigma_at v0) v0)"
+proof (rule TD_plain_Interp.partial_correctness)
+  show "TD_plain.solve_dom cfg_T_ip v0" by (fact dom)
+  show "TD_plain_Interp_solve cfg_T_ip v0 = td_sigma_at v0"
+    by (simp add: td_sigma_at_solve)
+qed
+
+lemma td_env_at_eq_le:
+  assumes dom: "TD_plain.solve_dom cfg_T_ip v0"
+  assumes w_reach: "w \<in> reach cfg_T_ip (td_sigma_at v0) v0"
+  shows "(eq cfg_T_ip) w (td_sigma_at v0) \<le> mlup (td_sigma_at v0) w"
+  using part_solutionD[OF td_plain_part_solution_at[OF dom] w_reach] by simp
+
+lemma td_sigma_at_eq_le_on_reach:
+  assumes dom: "TD_plain.solve_dom cfg_T_ip v0"
+  assumes v_reach: "v \<in> reach cfg_T_ip (td_sigma_at v0) v0"
+  shows "(eq cfg_T_ip) v (td_sigma_at v0) \<le> mlup (td_sigma_at v0) v"
+  using td_env_at_eq_le[OF dom v_reach] by simp
+
+lemma td_env_at_rhs_ip_le:
+  assumes cfi: "comp_fun_idem join_abs"
+  assumes join_sym: "\<And>x y. join_abs x y = join_abs y x"
+  assumes dom: "TD_plain.solve_dom cfg_T_ip v0"
+  assumes w_reach: "w \<in> reach cfg_T_ip (td_sigma_at v0) v0"
+  shows "rhs_ip g tf join_abs bot_abs s0 (td_env_at v0) w \<le> td_env_at v0 w"
+proof -
+  have eq_le: "(eq cfg_T_ip) w (td_sigma_at v0) \<le> mlup (td_sigma_at v0) w"
+    using td_env_at_eq_le[OF dom w_reach] .
+  show ?thesis
+    using eq_le_mlup_imp_rhs_ip_le[OF cfg_T_ip_eq fin fin_combines cfi join_sym eq_le]
+      unfolding td_env_at_def by simp
+qed
+
+lemma td_env_at_entry_le_ip:
+  assumes cfi: "comp_fun_idem join_abs"
+  assumes join_sym: "\<And>x y. join_abs x y = join_abs y x"
+  assumes join_is_sup: "join_abs = (\<squnion>)"
+  assumes bot_is_bot: "bot_abs = bot"
+  assumes dom: "TD_plain.solve_dom cfg_T_ip v0"
+  assumes entry_path: "cfg_path g (cfg_entry g) es v0"
+  shows "s0 \<le> td_env_at v0 (cfg_entry g)"
+proof -
+  have entry_reach: "cfg_entry g \<in> reach cfg_T_ip (td_sigma_at v0) v0"
+    using cfg_path_node_in_reach_ip[OF entry_path] .
+  have rhs_le: "rhs_ip g tf join_abs bot_abs s0 (td_env_at v0) (cfg_entry g)
+    \<le> td_env_at v0 (cfg_entry g)"
+    using td_env_at_rhs_ip_le[OF cfi join_sym dom entry_reach] .
+  have s0_rhs: "s0 \<le> rhs_ip g tf join_abs bot_abs s0 (td_env_at v0) (cfg_entry g)"
+    by (smt (verit, ccfv_SIG) bot_is_bot fin fin_combines join_is_sup order_trans rhs_le_rhs_ip
+        s0_le_rhs_entry)
+  show ?thesis using order_trans[OF s0_rhs rhs_le] .
+qed
+
+lemma td_env_at_path_step_le_ip:
+  assumes cfi: "comp_fun_idem join_abs"
+  assumes join_sym: "\<And>x y. join_abs x y = join_abs y x"
+  assumes join_is_sup: "join_abs = (\<squnion>)"
+  assumes bot_is_bot: "bot_abs = bot"
+  assumes dom: "TD_plain.solve_dom cfg_T_ip v0"
+  assumes path: "cfg_path g u ((a, w) # es') v0"
+  shows "apply_tf tf a (td_env_at v0 u) \<le> td_env_at v0 w"
+proof -
+  from path obtain ed: "(u, a, w) \<in> edges g" and p2: "cfg_path g w es' v0"
+    by (cases rule: cfg_path.cases) auto
+  have w_reach: "w \<in> reach cfg_T_ip (td_sigma_at v0) v0"
+    using cfg_path_node_in_reach_ip[OF p2] .
+  have le_rhs: "apply_tf tf a (td_env_at v0 u)
+    \<le> rhs_ip g tf join_abs bot_abs s0 (td_env_at v0) w"
+    using apply_tf_le_rhs_ip[where env="td_env_at v0", OF fin fin_combines ed]
+      join_is_sup bot_is_bot by (simp add: join_is_sup bot_is_bot)
+  show ?thesis
+    using order_trans[OF le_rhs td_env_at_rhs_ip_le[OF cfi join_sym dom w_reach]] .
+qed
+
+lemma td_env_at_edge_step_le_ip:
+  assumes cfi: "comp_fun_idem join_abs"
+  assumes join_sym: "\<And>x y. join_abs x y = join_abs y x"
+  assumes join_is_sup: "join_abs = (\<squnion>)"
+  assumes bot_is_bot: "bot_abs = bot"
+  assumes dom: "TD_plain.solve_dom cfg_T_ip v0"
+  assumes ed: "(u, a, w) \<in> edges g"
+  assumes w_reach: "w \<in> reach cfg_T_ip (td_sigma_at v0) v0"
+  shows "apply_tf tf a (td_env_at v0 u) \<le> td_env_at v0 w"
+proof -
+  have le_rhs: "apply_tf tf a (td_env_at v0 u)
+    \<le> rhs_ip g tf join_abs bot_abs s0 (td_env_at v0) w"
+    using apply_tf_le_rhs_ip[where env="td_env_at v0", OF fin fin_combines ed]
+      join_is_sup bot_is_bot by (simp add: join_is_sup bot_is_bot)
+  show ?thesis
+    using order_trans[OF le_rhs td_env_at_rhs_ip_le[OF cfi join_sym dom w_reach]] .
+qed
+
+lemma td_env_at_combine_le_ip:
+  assumes cfi: "comp_fun_idem join_abs"
+  assumes join_sym: "\<And>x y. join_abs x y = join_abs y x"
+  assumes join_is_sup: "join_abs = (\<squnion>)"
+  assumes bot_is_bot: "bot_abs = bot"
+  assumes dom: "TD_plain.solve_dom cfg_T_ip v0"
+  assumes uce: "(c, ex, w) \<in> combines g"
+  assumes w_reach: "w \<in> reach cfg_T_ip (td_sigma_at v0) v0"
+  shows "combine_abs (td_env_at v0 c) (td_env_at v0 ex) \<le> td_env_at v0 w"
+proof -
+  have le_rhs: "combine_abs (td_env_at v0 c) (td_env_at v0 ex)
+    \<le> rhs_ip g tf join_abs bot_abs s0 (td_env_at v0) w"
+    using combine_abs_le_rhs_ip[where env="td_env_at v0", OF fin fin_combines uce]
+      join_is_sup bot_is_bot
+    by (simp add: join_is_sup bot_is_bot)
+  show ?thesis
+    using order_trans[OF le_rhs td_env_at_rhs_ip_le[OF cfi join_sym dom w_reach]] .
+qed
+
+lemma td_env_at_entry_le_ip_reach:
+  assumes cfi: "comp_fun_idem join_abs"
+  assumes join_sym: "\<And>x y. join_abs x y = join_abs y x"
+  assumes join_is_sup: "join_abs = (\<squnion>)"
+  assumes bot_is_bot: "bot_abs = bot"
+  assumes dom: "TD_plain.solve_dom cfg_T_ip v0"
+  assumes entry_reach: "cfg_entry g \<in> reach cfg_T_ip (td_sigma_at v0) v0"
+  shows "s0 \<le> td_env_at v0 (cfg_entry g)"
+proof -
+  have rhs_le: "rhs_ip g tf join_abs bot_abs s0 (td_env_at v0) (cfg_entry g)
+    \<le> td_env_at v0 (cfg_entry g)"
+    using td_env_at_rhs_ip_le[OF cfi join_sym dom entry_reach] .
+  have s0_rhs: "s0 \<le> rhs_ip g tf join_abs bot_abs s0 (td_env_at v0) (cfg_entry g)"
+  proof -
+    have "s0 \<le> rhs g tf join_abs bot_abs s0 (td_env_at v0) (cfg_entry g)"
+      using s0_le_rhs_entry[where env="td_env_at v0", OF fin] join_is_sup bot_is_bot
+      by (simp add: join_is_sup bot_is_bot)
+    also have "\<dots> \<le> rhs_ip g tf join_abs bot_abs s0 (td_env_at v0) (cfg_entry g)"
+      using rhs_le_rhs_ip[OF fin fin_combines] by (simp add: join_is_sup bot_is_bot)
+    finally show ?thesis .
+  qed
+  show ?thesis using order_trans[OF s0_rhs rhs_le] .
+qed
+
+(* cfg_env_post_fixpoint_ip_from_solver needs eq \<le> mlup at every pp; TD_plain
+   only yields equality on dependency reach from v0.  Soundness at a query node
+   should follow the path-based post_fixpoint_sound_at_ip route (see TD_Soundness),
+   not this lemma. *)
+
+end
+
+definition td_analyse_ip ::
+    "proc_table
+     \<Rightarrow> pname list
+     \<Rightarrow> pcom
+     \<Rightarrow> 'a::bounded_semilattice_sup_bot domain_transfer
+     \<Rightarrow> ('a abs_state \<Rightarrow> 'a abs_state \<Rightarrow> 'a abs_state)
+     \<Rightarrow> 'a abs_state
+     \<Rightarrow> 'a abs_state
+     \<Rightarrow> pp
+     \<Rightarrow> 'a abs_state"
+where
+  "td_analyse_ip pi ps main tf join_abs bot_abs s0 v =
+     lookup_bot (TD_plain_Interp_solve
+       (make_rhs_tree_ip (compile_prog pi ps main) tf join_abs bot_abs s0) v) v"
+
+lemma td_analyse_ip_def_expand:
+  "td_analyse_ip pi ps main tf join_abs bot_abs s0 v =
+     lookup_bot (TD_plain_Interp_solve
+       (make_rhs_tree_ip (compile_prog pi ps main) tf join_abs bot_abs s0) v) v"
+  unfolding td_analyse_ip_def by simp
+
+lemma td_analyse_ip_eq_env_at:
+  fixes pi ps main and tf :: "'a::bounded_semilattice_sup_bot domain_transfer"
+    and join_abs :: "'a abs_state \<Rightarrow> 'a abs_state \<Rightarrow> 'a abs_state"
+    and bot_abs s0 :: "'a abs_state" and v
+  shows "td_analyse_ip pi ps main tf join_abs bot_abs s0 v =
+         td_cfg_ip_solver.td_env_at (compile_prog pi ps main) tf join_abs bot_abs s0 v v"
+proof -
+  interpret ip: td_cfg_ip_solver "compile_prog pi ps main" tf join_abs bot_abs s0
+    using compile_prog_finite td_cfg_ip_core_def td_cfg_ip_solver.intro by blast 
+  
+  show ?thesis
+    unfolding td_analyse_ip_def ip.td_env_at_def ip.td_sigma_at_def ip.cfg_T_ip_def by simp
 qed
 
 end
