src/Solver/TD_IP_Soundness.thy
@@ -1,0 +1,191 @@
+theory TD_IP_Soundness
+  imports TD_Interface Constraint_System_IP_Sound Sign_Domain CFG_Collect_IP_Adeq
+begin
+
+context sound_domain
+begin
+
+theorem td_analyse_ip_collect_sound_at:
+  fixes pi ps main v0
+  assumes tf_sound_assign:
+    "\<forall>x a sigma. \<forall>s \<in> gamma_state sigma.
+       s(x := aval a s) \<in> gamma_state (tf_assign tf x a sigma)"
+  assumes tf_sound_assume:
+    "\<forall>b sigma. \<forall>s \<in> gamma_state sigma. bval b s
+       \<longrightarrow> s \<in> gamma_state (tf_assume tf b sigma)"
+  assumes tf_sound_assume_not:
+    "\<forall>b sigma. \<forall>s \<in> gamma_state sigma. \<not> bval b s
+       \<longrightarrow> s \<in> gamma_state (tf_assume_not tf b sigma)"
+  assumes tf_sound_enter:
+    "\<forall>sigma. \<forall>s \<in> gamma_state sigma.
+       enter_state s \<in> gamma_state (tf_enter tf sigma)"
+  assumes S_sub: "S \<le> gamma_state s0"
+  assumes fin_cfg: "finite (edges (compile_prog pi ps main))"
+  assumes fin_comb: "finite (combines (compile_prog pi ps main))"
+  assumes td_solve_dom:
+    "TD_plain.solve_dom (make_rhs_tree_ip (compile_prog pi ps main) tf (\<squnion>) bot s0) v0"
+  assumes edge_reach:
+    "\<And>u a w. (u, a, w) \<in> edges (compile_prog pi ps main)
+       \<Longrightarrow> w \<in> reach (make_rhs_tree_ip (compile_prog pi ps main) tf (\<squnion>) bot s0)
+         (TD_plain_Interp_solve (make_rhs_tree_ip (compile_prog pi ps main) tf (\<squnion>) bot s0) v0) v0"
+  assumes combine_reach:
+    "\<And>c ex w. (c, ex, w) \<in> combines (compile_prog pi ps main)
+       \<Longrightarrow> w \<in> reach (make_rhs_tree_ip (compile_prog pi ps main) tf (\<squnion>) bot s0)
+         (TD_plain_Interp_solve (make_rhs_tree_ip (compile_prog pi ps main) tf (\<squnion>) bot s0) v0) v0"
+  assumes entry_reach:
+    "cfg_entry (compile_prog pi ps main)
+     \<in> reach (make_rhs_tree_ip (compile_prog pi ps main) tf (\<squnion>) bot s0)
+       (TD_plain_Interp_solve (make_rhs_tree_ip (compile_prog pi ps main) tf (\<squnion>) bot s0) v0) v0"
+  shows "cfg_collect_ip (compile_prog pi ps main) S v0
+         \<le> gamma_state (td_analyse_ip pi ps main tf (\<squnion>) bot s0 v0)"
+proof -
+  define g where "g = compile_prog pi ps main"
+  have fin_g: "finite (edges g)" unfolding g_def using fin_cfg by simp
+  have finC_g: "finite (combines g)" unfolding g_def using fin_comb by simp
+  interpret ip: td_cfg_ip_solver g tf "(\<squnion>)" bot s0
+    using fin_g finC_g td_cfg_ip_core_def td_cfg_ip_solver.intro by blast
+  define env where "env = ip.td_env_at v0"
+  have cfi: "comp_fun_idem ((\<squnion>) :: 'a abs_state \<Rightarrow> _ \<Rightarrow> _)"
+    by (rule join_state_comp_fun_idem)
+  have join_sym: "\<And>x y :: 'a abs_state. x \<squnion> y = y \<squnion> x"
+    by (rule sup.commute)
+  have join_is_sup: "(\<squnion>) = (\<squnion>)" by simp
+  have bot_is_bot: "bot = bot" by simp
+  have cfg_T_ip_fn: "ip.cfg_T_ip = make_rhs_tree_ip g tf (\<squnion>) bot s0"
+    by (simp add: ip.cfg_T_ip_def fun_eq_iff)
+  have reach_tree: "reach ip.cfg_T_ip = reach (make_rhs_tree_ip g tf (\<squnion>) bot s0)"
+    unfolding cfg_T_ip_fn by simp
+  have sigma_solve: "ip.td_sigma_at v0 = TD_plain_Interp_solve (make_rhs_tree_ip g tf (\<squnion>) bot s0) v0"
+    unfolding ip.td_sigma_at_def ip.td_sigma_at_solve cfg_T_ip_fn by simp
+  have dom: "TD_plain.solve_dom ip.cfg_T_ip v0"
+  proof -
+    have "TD_plain.solve_dom (make_rhs_tree_ip g tf (\<squnion>) bot s0) v0"
+      unfolding g_def by (rule td_solve_dom)
+    thus ?thesis unfolding cfg_T_ip_fn by simp
+  qed
+  have step_le:
+    "\<And>u a w. (u, a, w) \<in> edges g \<Longrightarrow> apply_tf tf a (env u) \<le> env w"
+  proof -
+    fix u a w
+    assume ed: "(u, a, w) \<in> edges g"
+    have ed': "(u, a, w) \<in> edges (compile_prog pi ps main)"
+      using ed by (simp add: g_def)
+    have w_reach': "w \<in> reach (make_rhs_tree_ip g tf (\<squnion>) bot s0)
+        (TD_plain_Interp_solve (make_rhs_tree_ip g tf (\<squnion>) bot s0) v0) v0"
+      using edge_reach[OF ed'] by (simp add: g_def)
+    have w_reach: "w \<in> reach ip.cfg_T_ip (ip.td_sigma_at v0) v0"
+      using w_reach' unfolding reach_tree sigma_solve by simp
+    show "apply_tf tf a (env u) \<le> env w"
+      using ip.td_env_at_edge_step_le_ip[OF cfi join_sym join_is_sup bot_is_bot dom ed w_reach]
+      unfolding env_def .
+  qed
+  have combine_le:
+    "\<And>c ex ret. (c, ex, ret) \<in> combines g \<Longrightarrow> combine_abs (env c) (env ex) \<le> env ret"
+  proof -
+    fix c ex ret
+    assume uce: "(c, ex, ret) \<in> combines g"
+    have uce': "(c, ex, ret) \<in> combines (compile_prog pi ps main)"
+      using uce by (simp add: g_def)
+    have w_reach': "ret \<in> reach (make_rhs_tree_ip g tf (\<squnion>) bot s0)
+        (TD_plain_Interp_solve (make_rhs_tree_ip g tf (\<squnion>) bot s0) v0) v0"
+      using combine_reach[OF uce'] by (simp add: g_def)
+    have w_reach: "ret \<in> reach ip.cfg_T_ip (ip.td_sigma_at v0) v0"
+      using w_reach' unfolding reach_tree sigma_solve by simp
+    show "combine_abs (env c) (env ex) \<le> env ret"
+      using ip.td_env_at_combine_le_ip[OF cfi join_sym join_is_sup bot_is_bot dom uce w_reach]
+      unfolding env_def .
+  qed
+  have entry_reach': "cfg_entry g \<in> reach ip.cfg_T_ip (ip.td_sigma_at v0) v0"
+  proof -
+    have er: "cfg_entry g \<in> reach (make_rhs_tree_ip g tf (\<squnion>) bot s0)
+        (TD_plain_Interp_solve (make_rhs_tree_ip g tf (\<squnion>) bot s0) v0) v0"
+      using entry_reach by (simp add: g_def)
+    show ?thesis using er unfolding reach_tree sigma_solve by simp
+  qed
+  have entry_le: "s0 \<le> env (cfg_entry g)"
+    using ip.td_env_at_entry_le_ip_reach[OF cfi join_sym join_is_sup bot_is_bot dom entry_reach']
+    unfolding env_def .
+  have collect_le: "cfg_collect_ip g S v0 \<le> gamma_state (env v0)"
+  proof (rule post_fixpoint_sound_at_ip)
+    show "finite (edges g)" by (rule fin_g)
+    show "finite (combines g)" by (rule finC_g)
+    show "S \<le> gamma_state s0" by (rule S_sub)
+    show "\<And>u a w. (u, a, w) \<in> edges g \<Longrightarrow> apply_tf tf a (env u) \<le> env w"
+      by (rule step_le)
+    show "\<And>c ex ret. (c, ex, ret) \<in> combines g \<Longrightarrow>
+        combine_abs (env c) (env ex) \<le> env ret"
+      by (rule combine_le)
+    show "s0 \<le> env (cfg_entry g)" by (rule entry_le)
+    show "\<forall>x a sigma. \<forall>s \<in> gamma_state sigma.
+        s(x := aval a s) \<in> gamma_state (tf_assign tf x a sigma)"
+      by (rule tf_sound_assign)
+    show "\<forall>b sigma. \<forall>s \<in> gamma_state sigma. bval b s
+        \<longrightarrow> s \<in> gamma_state (tf_assume tf b sigma)"
+      by (rule tf_sound_assume)
+    show "\<forall>b sigma. \<forall>s \<in> gamma_state sigma. \<not> bval b s
+        \<longrightarrow> s \<in> gamma_state (tf_assume_not tf b sigma)"
+      by (rule tf_sound_assume_not)
+    show "\<forall>sigma. \<forall>s \<in> gamma_state sigma.
+        enter_state s \<in> gamma_state (tf_enter tf sigma)"
+      by (rule tf_sound_enter)
+  qed
+  show ?thesis
+    using collect_le by (simp add: env_def g_def td_analyse_ip_eq_env_at)
+qed
+
+theorem ip_sign_analysis_sound:
+  fixes pi ps main and s t :: store and s0 :: "'a abs_state"
+  assumes tf_sound_assign:
+    "\<forall>x a sigma. \<forall>st \<in> gamma_state sigma.
+       st(x := aval a st) \<in> gamma_state (tf_assign tf x a sigma)"
+  assumes tf_sound_assume:
+    "\<forall>b sigma. \<forall>st \<in> gamma_state sigma. bval b st
+       \<longrightarrow> st \<in> gamma_state (tf_assume tf b sigma)"
+  assumes tf_sound_assume_not:
+    "\<forall>b sigma. \<forall>st \<in> gamma_state sigma. \<not> bval b st
+       \<longrightarrow> st \<in> gamma_state (tf_assume_not tf b sigma)"
+  assumes tf_sound_enter:
+    "\<forall>sigma. \<forall>st \<in> gamma_state sigma.
+       enter_state st \<in> gamma_state (tf_enter tf sigma)"
+  assumes s_sound: "s \<in> gamma_state s0"
+  assumes collect_exit:
+    "t \<in> cfg_collect_ip (compile_prog pi ps main) {s}
+       (cfg_exit (compile_prog pi ps main))"
+  assumes fin_cfg: "finite (edges (compile_prog pi ps main))"
+  assumes fin_comb: "finite (combines (compile_prog pi ps main))"
+  assumes td_solve_dom:
+    "TD_plain.solve_dom (make_rhs_tree_ip (compile_prog pi ps main) tf (\<squnion>) bot s0)
+       (cfg_exit (compile_prog pi ps main))"
+  assumes edge_reach:
+    "\<And>u a w. (u, a, w) \<in> edges (compile_prog pi ps main)
+       \<Longrightarrow> w \<in> reach (make_rhs_tree_ip (compile_prog pi ps main) tf (\<squnion>) bot s0)
+         (TD_plain_Interp_solve (make_rhs_tree_ip (compile_prog pi ps main) tf (\<squnion>) bot s0)
+           (cfg_exit (compile_prog pi ps main))) (cfg_exit (compile_prog pi ps main))"
+  assumes combine_reach:
+    "\<And>c ex w. (c, ex, w) \<in> combines (compile_prog pi ps main)
+       \<Longrightarrow> w \<in> reach (make_rhs_tree_ip (compile_prog pi ps main) tf (\<squnion>) bot s0)
+         (TD_plain_Interp_solve (make_rhs_tree_ip (compile_prog pi ps main) tf (\<squnion>) bot s0)
+           (cfg_exit (compile_prog pi ps main))) (cfg_exit (compile_prog pi ps main))"
+  assumes entry_reach:
+    "cfg_entry (compile_prog pi ps main)
+     \<in> reach (make_rhs_tree_ip (compile_prog pi ps main) tf (\<squnion>) bot s0)
+       (TD_plain_Interp_solve (make_rhs_tree_ip (compile_prog pi ps main) tf (\<squnion>) bot s0)
+         (cfg_exit (compile_prog pi ps main))) (cfg_exit (compile_prog pi ps main))"
+  shows "t \<in> gamma_state
+       (td_analyse_ip pi ps main tf (\<squnion>) bot s0
+         (cfg_exit (compile_prog pi ps main)))"
+proof -
+  have S_sub: "{s} \<le> gamma_state s0" using s_sound by auto
+  have collect:
+    "cfg_collect_ip (compile_prog pi ps main) {s} (cfg_exit (compile_prog pi ps main))
+     \<le> gamma_state (td_analyse_ip pi ps main tf (\<squnion>) bot s0
+         (cfg_exit (compile_prog pi ps main)))"
+    by (rule td_analyse_ip_collect_sound_at[OF tf_sound_assign tf_sound_assume
+          tf_sound_assume_not tf_sound_enter S_sub fin_cfg fin_comb td_solve_dom
+          edge_reach combine_reach entry_reach])
+  show ?thesis using collect collect_exit by blast
+qed
+
+end
+
+end
